pipit/plugin-test/Plugin.Test.Core.Check.fst
@@ -6,7 +6,7 @@ open Pipit.Source
 
 module PPL = Pipit.Plugin.Lift
 // module PPC = Pipit.Plugin.Check
-module PSSB = Pipit.Sugar.Shallow.Base
+module PSSB = Pipit.Prim.HasStream
 
 module PPS  = Pipit.Prim.Shallow
 module PPT  = Pipit.Prim.Table
